Just updating to latest from dsl branch with kernel state.

compiler/dsl/coq/Reflex.v
@@ -1,7 +1,8 @@
-Require Import List.
 Require Import Ascii.
-Require Import String.
+Require Import Eqdep_dec.
 Require Import NPeano.
+Require Import List.
+Require Import String.
 Require Import Ynot.
 
 Require Import ReflexBase.
@@ -15,6 +16,8 @@ Open Scope char_scope.
 Open Scope hprop_scope.
 Open Scope stsepi_scope.
 Open Scope list_scope.
+
+Axiom TODO' : False. Definition TODO {A : Type} : A := match TODO' with end.
 
 Ltac sep' := sep fail idtac.
 Ltac inv H := inversion H; subst; clear H.
@@ -32,7 +35,23 @@ Qed.
 
 Inductive desc : Set := num_d | str_d | fd_d.
 
-Definition sdenote_desc (d : desc) : Set :=
+Definition desc_eqdec : forall x y : desc, decide (x = y).
+Proof.
+  decide equality.
+Qed.
+
+Module DecidableTypeDesc <: DecidableType.
+  Definition U := desc.
+  Definition eq_dec := desc_eqdec.
+End DecidableTypeDesc.
+
+Module DecidableEqDepDesc := DecidableEqDep(DecidableTypeDesc).
+
+Definition UIP_refl_desc :
+  forall (d : desc) (e : d = d), e = Logic.eq_refl d :=
+  DecidableEqDepDesc.UIP_refl.
+
+Fixpoint sdenote_desc (d : desc) : Set :=
   match d with
   | num_d => num
   | str_d => str
@@ -44,34 +63,34 @@ Instance SDenoted_desc : SDenoted desc :=
 { sdenote := sdenote_desc
 }.
 
-Definition payload_desc' n : Set := svec desc n.
+Definition vdesc' n : Set := svec desc n.
 
-Definition sdenote_payload_desc' n (pt : payload_desc' n) : Set :=
+Definition sdenote_vdesc' n (pt : vdesc' n) : Set :=
   shvec sdenote_desc pt.
 
-Instance SDenoted_payload_desc' { n } : SDenoted (payload_desc' n) :=
-{ sdenote := sdenote_payload_desc' n
+Instance SDenoted_vdesc' {n} : SDenoted (vdesc' n) :=
+{ sdenote := sdenote_vdesc' n
 }.
 
 (* Thank you Ynot for breaking sigT notation... *)
-Definition payload_desc := (sigT (fun (n : nat) => payload_desc' n)).
+Definition vdesc := (sigT (fun (n : nat) => vdesc' n)).
 
-Instance SDenoted_payload_desc : SDenoted payload_desc :=
-{ sdenote := fun pd => @sdenote _ (@SDenoted_payload_desc' (projT1 pd)) (projT2 pd)
+Definition sdenote_vdesc (v : vdesc) : Set :=
+  sdenote_vdesc' (projT1 v) (projT2 v).
+
+Instance SDenoted_vdesc : SDenoted vdesc :=
+{ sdenote := sdenote_vdesc
 }.
 
-Definition payload_desc_vec n := vec payload_desc n.
+Definition vvdesc n := vec vdesc n.
 
 Section WITH_PAYLOAD_DESC_VEC.
 
 Context {NB_MSG : nat}.
-Context {PDV : payload_desc_vec NB_MSG}.
+Context {VVD : vvdesc NB_MSG}.
 
-Definition lkup_tag (tag : fin NB_MSG) : payload_desc :=
-  vec_ith PDV tag.
-
-Definition sdenote_payload_desc (pd : payload_desc) : Set :=
-  sdenote_payload_desc' (projT1 pd) (projT2 pd).
+Definition lkup_tag (tag : fin NB_MSG) : vdesc :=
+  vec_ith VVD tag.
 
 Record msg : Set :=
   { tag : fin NB_MSG
@@ -103,44 +122,38 @@ Section WITH_TRACE_FUN.
 
 Variable trace_fun : fd -> forall (d : desc), s[[ d ]] -> list Action.
 
-Fixpoint trace_payload_desc'
-  (n : nat) (pd : payload_desc' n) (f : fd) (p : s[[ pd ]]) : Trace :=
-  match n as _n return
-    forall (pd : payload_desc' _n) (p : s[[ pd ]]), Trace
-  with
+Fixpoint trace_payload' (f : fd) (n : nat) :
+  forall (pd : vdesc' n) (p : s[[ pd ]]), Trace :=
+  match n with
   | O => fun _ _ => nil
-  | S n' => fun (pd : payload_desc' (S n')) (p : s[[ pd ]]) =>
-    match pd as _pd return
-      forall (p : @sdenote _ (@SDenoted_payload_desc' (S n')) _pd), Trace
-    with
-    | (d, pd') => fun p => trace_payload_desc' n' pd' f (snd p) ++ trace_fun f d (fst p)
-    end p
-  end pd p
-.
+  | S n' => fun pd =>
+    let (d, pd') as _pd return forall (p : sdenote_vdesc' (S n') _pd), _ := pd in
+    fun p => trace_payload' f n' pd' (snd p) ++ trace_fun f d (fst p)
+  end.
 
-Definition trace_payload_desc (pd : payload_desc) :=
-  trace_payload_desc' (projT1 pd) (projT2 pd).
+Definition trace_payload (pd : vdesc) (f : fd) :=
+  trace_payload' f (projT1 pd) (projT2 pd).
 
-Definition trace_opt_payload_desc (opd : option payload_desc) (f : fd)
+Definition trace_opt_payload (opd : option vdesc) (f : fd)
   : s[! opd !] -> Trace :=
   match opd as _opd return s[! _opd !] -> Trace with
   | None => fun p => match p with end
-  | Some spt => fun p => trace_payload_desc spt f p
+  | Some spt => fun p => trace_payload spt f p
   end.
 
 End WITH_TRACE_FUN.
 
-Definition trace_payload_recv' := trace_payload_desc' trace_recv.
+Definition trace_payload_recv' := trace_payload' trace_recv.
 
-Definition trace_payload_send' := trace_payload_desc' trace_send.
+Definition trace_payload_send' := trace_payload' trace_send.
 
-Definition trace_payload_recv := trace_payload_desc trace_recv.
+Definition trace_payload_recv := trace_payload trace_recv.
 
-Definition trace_payload_send := trace_payload_desc trace_send.
+Definition trace_payload_send := trace_payload trace_send.
 
-Definition trace_opt_payload_recv := trace_opt_payload_desc trace_recv.
+Definition trace_opt_payload_recv := trace_opt_payload trace_recv.
 
-Definition trace_opt_payload_send := trace_opt_payload_desc trace_send.
+Definition trace_opt_payload_send := trace_opt_payload trace_send.
 
 Definition trace_recv_msg (f : fd) (m : msg) : Trace :=
   let t := tag m in
@@ -159,21 +172,28 @@ Definition trace_send_msg (f : fd) (m : msg) : Trace :=
   let t := tag m in
   trace_payload_send (lkup_tag t) f (pay m) ++ SendNum f (num_of_fin t).
 
+Definition open_if_fd (t : desc) : s[[ t ]] -> hprop :=
+  match t as _t return s[[ _t ]] -> hprop with
+  | fd_d => fun v => open v | _ => fun _ => emp
+  end.
+
 Definition recv_arg :
-  forall (f : fd) (ps : list Perm) (t : desc) (tr : [Trace]),
-  STsep (tr ~~ traced tr * open f ps * [In RecvP ps] * [In RecvFDP ps])
-        (fun v : s[[ t ]] => tr ~~ traced (trace_recv f t v ++ tr) * open f ps).
+  forall (f : fd) (t : desc) (tr : [Trace]),
+  STsep (tr ~~ traced tr * open f)
+        (fun v : s[[ t ]] => tr ~~
+          traced (trace_recv f t v ++ tr) * open f * open_if_fd _ v
+        ).
 Proof.
   intros; refine (
     match t as _t return STsep _ (fun v : s[[ _t ]] => _) with
     | num_d =>
-      n <- recv_num f ps tr;
+      n <- recv_num f tr;
       {{ Return n }}
     | str_d =>
-      s <- recv_str f ps tr;
+      s <- recv_str f tr;
       {{ Return s }}
     | fd_d =>
-      g <- recv_fd f ps tr;
+      g <- recv_fd f tr;
       {{ Return g }}
     end
   );
@@ -181,9 +201,9 @@ Proof.
 Qed.
 
 Definition send_arg :
-  forall (f : fd) (ps : list Perm) (d : desc) (v : s[[ d ]]) (tr : [Trace]),
-  STsep (tr ~~ traced tr * open f ps * [In SendP ps] * [In SendFDP ps])
-        (fun _ : unit => tr ~~ traced (trace_send f d v ++ tr) * open f ps).
+  forall (f : fd) (d : desc) (v : s[[ d ]]) (tr : [Trace]),
+  STsep (tr ~~ traced tr * open f)
+        (fun _ : unit => tr ~~ traced (trace_send f d v ++ tr) * open f).
 Proof.
   intros; refine (
     match d as _d return
@@ -191,89 +211,112 @@ Proof.
       STsep _ (fun _ => tr ~~ traced (trace_send f _d v ++ tr) * _)
     with
     | num_d => fun v =>
-      send_num f ps v tr;;
+      send_num f v tr;;
       {{ Return tt }}
     | str_d => fun v =>
-      send_str f ps v tr;;
+      send_str f v tr;;
       {{ Return tt }}
     | fd_d => fun v =>
-      send_fd f ps v tr;;
+      send_fd f v tr;;
       {{ Return tt }}
     end v
   );
   sep'.
 Qed.
 
+Fixpoint all_open_payload' (n : nat) :
+  forall (v : vdesc' n), sdenote_vdesc' n v -> hprop :=
+  match n with
+  | 0 => fun _ _ => emp
+  | S n' => fun v =>
+    let (d, v') as _v return (sdenote_vdesc' (S n') _v -> hprop) := v in
+    match d with
+    | fd_d => fun vv =>
+      let (vd, vv') := vv in
+      open vd * all_open_payload' n' v' vv'
+    | _ => fun vv =>
+      let (_, vv') := vv in
+      all_open_payload' n' v' vv'
+    end
+  end.
+
+Definition all_open_payload {v : vdesc} : s[[ v ]] -> hprop :=
+  all_open_payload' (projT1 v) (projT2 v).
+
 Definition recv_payload' :
-  forall (f : fd) (ps : list Perm) (n : nat) (pd : payload_desc' n) (tr : [Trace]),
-  STsep (tr ~~ traced tr * open f ps * [In RecvP ps] * [In RecvFDP ps])
-        (fun pv : s[[ pd ]] =>
-           tr ~~ traced (trace_payload_recv' n pd f pv ++ tr) * open f ps).
+  forall (f : fd) (n : nat) (pd : vdesc' n) (tr : [Trace]),
+  STsep (tr ~~ traced tr * open f)
+        (fun pv : s[[ pd ]] => tr ~~
+          traced (trace_payload_recv' f n pd pv ++ tr) * open f
+          * all_open_payload' n pd pv
+        ).
 Proof.
   intros; refine (
     Fix3
-      (fun n pd tr => tr ~~ traced tr * open f ps * [In RecvP ps] * [In RecvFDP ps])
-      (fun n pd tr (pv : s[[ pd ]]) =>
-         tr ~~ traced (trace_payload_recv' n pd f pv ++ tr) * open f ps)
-      (fun self (n : nat) (pd : payload_desc' n) tr =>
+      (fun n pd tr => tr ~~ traced tr * open f)
+      (fun n pd tr (pv : s[[ pd ]]) => tr ~~
+        traced (trace_payload_recv' f n pd pv ++ tr) * open f
+        * all_open_payload' n pd pv)
+      (fun self (n : nat) (pd : vdesc' n) tr =>
          match n as _n return
-           forall (pd : payload_desc' _n), STsep _ (fun x : s[[ pd ]] => _)
+           forall (pd : vdesc' _n), STsep _ (fun x : s[[ pd ]] => _)
          with
          | O => fun _ => {{ Return tt }}
          | S n' => fun pt =>
            match pt with
            | (d, pt') =>
-             v  <- recv_arg f ps d tr <@> [In RecvP ps] * [In RecvFDP ps];
-             vs <- self n' pt' (tr ~~~ trace_recv f d v ++ tr);
+             v  <- recv_arg f d tr;
+             vs <- self n' pt' (tr ~~~ trace_recv f d v ++ tr) <@> open_if_fd _ v;
              {{ Return (v, vs) }}
            end
          end pd
       )
     n pd tr
-  );
-  sep'.
+  ); sep'.
   inv H; rewrite app_assoc; sep'.
+  destruct d; sep'.
 Qed.
 
 Definition recv_payload :
-  forall (f : fd) (ps : list Perm) (pd : payload_desc) (tr : [Trace]),
-  STsep (tr ~~ traced tr * open f ps * [In RecvP ps] * [In RecvFDP ps])
-        (fun pv : s[[ pd ]] =>
-           tr ~~ traced (trace_payload_recv pd f pv ++ tr) * open f ps).
+  forall (f : fd) (pd : vdesc) (tr : [Trace]),
+  STsep (tr ~~ traced tr * open f)
+        (fun pv : s[[ pd ]] => tr ~~
+          traced (trace_payload_recv pd f pv ++ tr) * open f
+          * all_open_payload pv
+        ).
 Proof.
-  intros f ps pd. destruct pd as [n pd].
-  exact (recv_payload' f ps n pd).
+  intros f pd. destruct pd as [n pd].
+  exact (recv_payload' f n pd).
 Qed.
 
 Definition send_payload' :
-  forall (f : fd) (ps : list Perm) (n : nat) (pd : payload_desc' n) (pv : s[[ pd ]])
+  forall (f : fd) (n : nat) (pd : vdesc' n) (pv : s[[ pd ]])
          (tr : [Trace]),
-  STsep (tr ~~ traced tr * open f ps * [In SendP ps] * [In SendFDP ps])
+  STsep (tr ~~ traced tr * open f)
         (fun _ : unit =>
-           tr ~~ traced (trace_payload_send' n pd f pv ++ tr) * open f ps).
+           tr ~~ traced (trace_payload_send' f n pd pv ++ tr) * open f).
 Proof.
   intros; refine (
     Fix4
-      (fun n pd pv tr => tr ~~ traced tr * open f ps * [In SendP ps] * [In SendFDP ps])
+      (fun n pd pv tr => tr ~~ traced tr * open f)
       (fun n pd pv (tr : [Trace]) _ =>
-         tr ~~ traced (trace_payload_send' n pd f pv ++ tr) * open f ps)
-      (fun self (n : nat) (pd : payload_desc' n) pv (tr : [Trace])
-       =>
+         tr ~~ traced (trace_payload_send' f n pd pv ++ tr) * open f)
+      (fun self (n : nat) (pd : vdesc' n) pv (tr : [Trace]) =>
          match n as _n return
-           forall (pd : payload_desc' _n) (pv : s[[ pd ]]),
+           forall (pd : vdesc' _n) (pv : s[[ pd ]]),
              STsep _ (fun _ =>
-                        tr ~~ traced (trace_payload_send' _n pd f pv ++ tr) * _)
+                        tr ~~ traced (trace_payload_send' f _n pd pv ++ tr) * _)
          with
          | O => fun _ _ => {{ Return tt }}
-         | S n' => fun (pd : payload_desc' (S n'))
-                       (pv : @sdenote _ (@SDenoted_payload_desc' (S n')) pd) =>
+         | S n' => fun (pd : vdesc' (S n'))
+                       (pv : sdenote_vdesc' (S n') pd) =>
            match pd as _pd return
-             forall (pv : @sdenote _ (@SDenoted_payload_desc' (S n')) _pd), STsep _ (fun _ => _)
+             forall (pv : sdenote_vdesc' (S n') _pd), STsep _ (fun _ => _)
            with
            | (d, pt') => fun pv =>
              match pv with
              | (v, pv') =>
-               send_arg f ps d v tr <@> [In SendP ps] * [In SendFDP ps];;
+               send_arg f d v tr;;
                self n' pt' pv' (tr ~~~ trace_send f d v ++ tr);;
                {{ Return tt }}
              end
@@ -285,26 +328,29 @@ Proof.
 Qed.
 
 Definition send_payload :
-  forall (f : fd) (ps : list Perm) (pd : payload_desc) (pv : s[[ pd ]]) (tr : [Trace]),
-  STsep (tr ~~ traced tr * open f ps * [In SendP ps] * [In SendFDP ps])
-        (fun _ : unit => tr ~~ traced (trace_payload_send pd f pv ++ tr) * open f ps).
+  forall (f : fd) (pd : vdesc) (pv : s[[ pd ]]) (tr : [Trace]),
+  STsep (tr ~~ traced tr * open f)
+        (fun _ : unit => tr ~~ traced (trace_payload_send pd f pv ++ tr) * open f).
 Proof.
-  intros f ps pd. destruct pd as [n pd].
-  exact (send_payload' f ps n pd).
+  intros f pd. destruct pd as [n pd].
+  exact (send_payload' f n pd).
 Qed.
 
 Definition recv_msg :
-  forall (f : fd) (ps : list Perm) (tr : [Trace]),
-  STsep (tr ~~ traced tr * open f ps * [In RecvP ps] * [In RecvFDP ps])
-        (fun m : maybe_msg => tr ~~ traced (trace_recv_maybe_msg f m ++ tr) * open f ps).
+  forall (f : fd) (tr : [Trace]),
+  STsep (tr ~~ traced tr * open f)
+        (fun m : maybe_msg => tr ~~
+          traced (trace_recv_maybe_msg f m ++ tr) * open f
+          * match m with inl msg => all_open_payload (pay msg) | inr bog => emp end
+        ).
 Proof.
   intros; refine (
-    t <- recv_num f ps tr <@> [In RecvP ps] * [In RecvFDP ps];
+    t <- recv_num f tr;
     let oft := opt_fin NB_MSG (nat_of_num t) in
     match oft with
     | inleft (existT ft pf) =>
       let pt := lkup_tag ft in
-      pv <- recv_payload f ps pt (tr ~~~ RecvNum f t ++ tr);
+      pv <- recv_payload f pt (tr ~~~ RecvNum f t ++ tr);
       {{ Return (inl _ (Build_msg ft pv)) }}
     | inright pf => {{ Return (inr _ (Build_bogus_msg t pf)) }}
     end
@@ -319,15 +365,15 @@ Proof.
 Qed.
 
 Definition send_msg :
-  forall (f : fd) (ps : list Perm) (m : msg) (tr : [Trace]),
-  STsep (tr ~~ traced tr * open f ps * [In SendP ps] * [In SendFDP ps])
-        (fun _ : unit => tr ~~ traced (trace_send_msg f m ++ tr) * open f ps).
+  forall (f : fd) (m : msg) (tr : [Trace]),
+  STsep (tr ~~ traced tr * open f)
+        (fun _ : unit => tr ~~ traced (trace_send_msg f m ++ tr) * open f).
 Proof.
   intros; refine (
     let t := tag m in
     let pt := lkup_tag t in
-    send_num f ps (num_of_fin t) tr <@> [In SendP ps] * [In SendFDP ps];;
-    send_payload f ps pt (pay m) (tr ~~~ SendNum f (num_of_fin t) ++ tr);;
+    send_num f (num_of_fin t) tr;;
+    send_payload f pt (pay m) (tr ~~~ SendNum f (num_of_fin t) ++ tr);;
     {{ Return tt }}
   );
   sep'.
@@ -363,10 +409,16 @@ Fixpoint expand_ktrace (kt : KTrace) : Trace :=
   | ka :: kas => expand_kaction ka ++ expand_ktrace kas
   end.
 
-Record kstate : Set :=
-  mkst { components : list fd
-       ; ktr : [KTrace]
-       }.
+Context {KST_DESC_SIZE : nat}.
+Variable KST_DESC' : vdesc' KST_DESC_SIZE.
+Definition KST_DESC_ := existT _ KST_DESC_SIZE KST_DESC'.
+
+Record kstate : Set := mkst
+  { kcs : list fd
+  ; ktr : [KTrace]
+  ; kst : s[[ KST_DESC_ ]]
+  ; kfd : list fd (* need to keep track of all the open fds... *)
+  }.
 
 Inductive unop : desc -> desc -> Set :=
 | Not : unop num_d num_d
@@ -412,27 +464,165 @@ Definition eval_binop
 
 Implicit Arguments eval_binop.
 
-Section WITH_ENV.
+(*
+Notation unop d := (existT (fun n => vdesc' n) 1 (d, tt)).
+Notation binop a b := (existT (fun n => vdesc' n) 2 (a, (b, tt))).
+
+Inductive op : vdesc -> desc -> Set :=
+(* unary *)
+| Not : op (unop num_d) num_d
+(* binary *)
+| Eq :  forall (d : desc), op (binop d d) num_d
+| Add : op (binop num_d num_d) num_d
+| Sub : op (binop num_d num_d) num_d
+| Mul : op (binop num_d num_d) num_d
+| Cat : op (binop str_d str_d) str_d
+.
+
+Definition eval_op {args res} (o : op args res) : s[[ args ]] -> s[[ res ]] :=
+  match o in op _args _res  return
+    sdenote_vdesc _args -> s[[ _res ]]
+  with
+  | Not => fun args =>
+    let (v, _) := args in
+    if num_eq v FALSE then TRUE else FALSE
+  | Eq d => fun args =>
+    match args with (v1, (v2, _)) =>
+      let teq : forall (x y : s[[ d ]]), {x = y} + {x <> y} :=
+        match d with
+        | num_d => num_eq
+        | str_d => str_eq
+        | fd_d  => fd_eq
+        end
+      in
+      if teq v1 v2 then TRUE else FALSE
+    end
+  | Add => fun args =>
+    match args with (v1, (v2, _)) =>
+      num_of_nat (plus (nat_of_num v1) (nat_of_num v2))
+    end
+  | Sub => fun args =>
+    match args with (v1, (v2, _)) =>
+      num_of_nat (minus (nat_of_num v1) (nat_of_num v2))
+    end
+  | Mul => fun args =>
+    match args with (v1, (v2, _)) =>
+      num_of_nat (mult (nat_of_num v1) (nat_of_num v2))
+    end
+  | Cat => fun args =>
+    match args with (v1, (v2, _)) =>
+      v1 ++ v2
+    end
+  end.
+*)
+
+Section WITHIN_HANDLER.
 
 Variable CST : kstate.
 Variable CFD : fd.
 Variable CMSG : msg.
 
-Let CPAY : payload_desc := lkup_tag (tag CMSG).
+Let CPAY : vdesc := lkup_tag (tag CMSG).
+
+Definition payload_ith (vd : vdesc) :
+  sdenote_vdesc vd -> forall (i : fin (projT1 vd)), s[[ svec_ith (projT2 vd) i ]] :=
+  match vd as _vd with existT n pd => fun p i =>
+    shvec_ith sdenote_desc pd p i
+  end.
 
 Definition msg_param_i (i : fin (projT1 CPAY)) : s[[ svec_ith (projT2 CPAY) i ]] :=
-  match CPAY as _CPAY return
-    forall (p : s[[ _CPAY ]]) (i : fin (projT1 _CPAY)), s[[ svec_ith (projT2 _CPAY) i ]]
-  with
-  | existT n pd => fun (p : s[[ existT _ n pd ]]) (i : fin n) =>
-    shvec_ith sdenote_desc pd p i
-  end (pay CMSG) i.
+  payload_ith CPAY (pay CMSG) i.
+
+Fixpoint all_open_payload_drop' (n : nat) :
+  forall (v : vdesc' n) (drop : fd), sdenote_vdesc' n v -> hprop :=
+  match n with
+  | 0 => fun _ _ _ => emp
+  | S n' => fun v drop =>
+    let (d, v') as _v return (sdenote_vdesc' (S n') _v -> hprop) := v in
+    match d with
+    | fd_d => fun vv =>
+      let (vd, vv') := vv in
+      if fd_eq vd drop
+      then all_open_payload' n' v' vv'
+      else open vd * all_open_payload_drop' n' v' drop vv'
+    | _ => fun vv =>
+      let (_, vv') := vv in
+      all_open_payload_drop' n' v' drop vv'
+    end
+  end.
+
+Definition all_open_payload_drop {v : vdesc} : fd -> s[[ v ]] -> hprop :=
+  all_open_payload_drop' (projT1 v) (projT2 v).
+
+Definition fd_in_payload' := shvec_in sdenote_desc desc_eqdec fd_d.
+Definition fd_in_payload f (vd : vdesc) p := fd_in_payload' f (projT1 vd) (projT2 vd) p.
+
+Lemma unpack_all_open_payload' :
+  forall (n : nat) (vd : vdesc' n) (p : s[[ vd ]]) (f : fd),
+  fd_in_payload' f n vd p ->
+  all_open_payload' n vd p ==> open f * all_open_payload_drop' n vd f p.
+Proof.
+  intros n vd p f IN. induction n.
+  contradiction.
+  simpl in vd. destruct vd as [d vd'].
+  simpl in p. destruct p as [v p'].
+  simpl in IN. destruct (desc_eqdec fd_d d).
+  simpl in *. destruct e. intuition.
+  subst. destruct (fd_eq f f); sep fail idtac.
+  destruct (fd_eq v f); sep fail idtac.
+  specialize (IHn _ _ H). eapply himp_trans. apply IHn. sep fail idtac.
+  simpl. destruct d; first [ exact (IHn _ _ IN) | congruence ].
+Qed.
+
+Lemma unpack_all_open_payload :
+  forall (vd : vdesc) (p : s[[ vd ]]) (f : fd),
+  fd_in_payload f vd p ->
+  all_open_payload p ==> open f * all_open_payload_drop f p.
+Proof.
+  intros vd p f IN.
+  pose proof (unpack_all_open_payload' (projT1 vd) (projT2 vd) p f IN).
+  exact H.
+Qed.
+
+Lemma repack_all_open_payload' :
+  forall (n : nat) (vd : vdesc' n) (p : s[[ vd ]]) (f : fd),
+  fd_in_payload' f n vd p ->
+  open f * all_open_payload_drop' n vd f p ==> all_open_payload' n vd p.
+Proof.
+  intros n vd p f IN. induction n.
+  contradiction.
+  simpl in vd. destruct vd as [d vd'].
+  simpl in p. destruct p as [v p'].
+  simpl in IN. destruct (desc_eqdec fd_d d).
+  simpl in *. destruct e. intuition.
+  subst. destruct (fd_eq f f); sep fail idtac.
+  destruct (fd_eq v f); sep fail idtac.
+  specialize (IHn _ _ H). eapply himp_trans; [ | apply IHn]. sep fail idtac.
+  simpl. destruct d; first [ exact (IHn _ _ IN) | congruence ].
+Qed.
+
+Lemma repack_all_open_payload :
+  forall (vd : vdesc) (p : s[[ vd ]]) (f : fd),
+  fd_in_payload f vd p ->
+  open f * all_open_payload_drop f p ==> all_open_payload p.
+Proof.
+  intros vd p f IN.
+  pose proof (repack_all_open_payload' (projT1 vd) (projT2 vd) p f IN).
+  exact H.
+Qed.
+
+Definition env_fds_in l (envd : vdesc) (env : s[[ envd ]]) : Prop :=
+  forall i,
+  match svec_ith (projT2 envd) i as _d return s[[ _d ]] -> Prop with
+  | fd_d => fun (f : s[[ fd_d ]]) => In f l
+  | _ => fun _ => True
+  end (payload_ith envd env i).
 
 Definition msg_fds_ok : Prop :=
   forall i,
   let d := svec_ith (projT2 CPAY) i in
   match d as _d return s[[ _d ]] -> Prop with
-  | fd_d => fun (f : s[[ fd_d ]]) => In f (components CST)
+  | fd_d => fun (f : s[[ fd_d ]]) => In f (kcs CST)
   | _ => fun _ => True
   end (msg_param_i i).
 
@@ -444,92 +634,44 @@ Proof.
   intros s. destruct CST as [comps ktr]. simpl in *. apply in_dec. exact fd_eq.
 Qed.
 
+(*
+Definition msg_fds_ok : hprop := all_open_payload (pay CMSG).
+
+Definition msg_fds_in : Prop := env_fds_in (components CST) CPAY (pay CMSG).
+
+Definition decide_msg_fds_in : decide msg_fds_in.
+Proof.
+  apply forall_fin. intros i. generalize (payload_ith CPAY (pay CMSG) i).
+  destruct (svec_ith (projT2 CPAY) i).
+  now left. now left.
+  intros s. destruct CST as [comps ktr]. simpl in *. apply in_dec. exact fd_eq.
+Qed.
+*)
+
+Section WITH_ENVD.
+
+Variable ENVD : vdesc.
+
 Inductive base_expr : desc -> Set :=
-(* no fd lit, otherwise would make lit ctor polymorphic *)
 | NLit : num -> base_expr num_d
 | SLit : str -> base_expr str_d
-| CurChan : base_expr fd_d
-| Param :
-  forall (i : fin (projT1 CPAY)),
-  base_expr (svec_ith (projT2 CPAY) i)
-| UnOp :
-  forall d1 d2,
-  unop d1 d2 ->
-  base_expr d1 ->
-  base_expr d2
-| BinOp :
-  forall d1 d2 d3,
-  binop d1 d2 d3 ->
-  base_expr d1 ->
-  base_expr d2 ->
-  base_expr d3
+| Var : forall (i : fin (projT1 ENVD)), base_expr (svec_ith (projT2 ENVD) i)
+| UnOp : forall d1 d2, unop d1 d2 -> base_expr d1 -> base_expr d2
+| BinOp : forall d1 d2 d3, binop d1 d2 d3 -> base_expr d1 -> base_expr d2 -> base_expr d3
 .
 
-Fixpoint eval_base_expr (d : desc) (e : base_expr d) : s[[ d ]] :=
-  match e in base_expr _d return s[[ _d ]] with
-  | NLit n => n
-  | SLit s => s
-  | CurChan => CFD
-  | Param i => msg_param_i i
-  | UnOp t1 t2 op e =>
-    let v := eval_base_expr t1 e in
-    eval_unop op v
-  | BinOp t1 t2 t3 op e1 e2 =>
-    let v1 := eval_base_expr t1 e1 in
-    let v2 := eval_base_expr t2 e2 in
-    eval_binop op v1 v2
-  end.
-
-Lemma base_expr_fd_in :
-  forall t e v,
-  msg_fds_ok ->
-  In CFD (components CST)->
-  eval_base_expr t e = v ->
-  match t as _t return (s[[ _t ]] -> Prop) with
-  | fd_d => fun f => In f (components CST)
-  | _ => fun _ => True
-  end v.
-Proof.
-  destruct e; simpl; intros; subst; auto.
-  specialize (H i); auto.
-  destruct d2; auto. inv u.
-  destruct d3; auto. inv b.
-Qed.
-
-Fixpoint payload_expr' (n : nat) (pd : payload_desc' n) : Type :=
-  match n as _n return payload_desc' _n -> Type with
+Fixpoint payload_expr' (n : nat) (pd : vdesc' n) : Type :=
+  match n as _n return vdesc' _n -> Type with
   | O => fun p => unit
-  | S n' => fun (pd : payload_desc' (S n')) =>
+  | S n' => fun (pd : vdesc' (S n')) =>
     match pd with
     | (d, pd') => base_expr d * payload_expr' n' pd'
     end
   end%type pd.
 
-Definition payload_expr (pd : payload_desc) : Type :=
-  payload_expr' (projT1 pd) (projT2 pd).
+Definition payload_expr pd := payload_expr' (projT1 pd) (projT2 pd).
 
-Fixpoint eval_payload_expr' (n : nat) (pd : payload_desc' n) (e : payload_expr' n pd)
-  : s[[ pd ]] :=
-  match n as _n return
-    forall (pd : payload_desc' _n) (e : payload_expr' _n pd), s[[ pd ]]
-  with
-  | O => fun pd e => tt
-  | S n' => fun (pd : payload_desc' (S n')) (e : payload_expr' (S n') pd) =>
-    match pd as _pd return payload_expr' (S n') _pd -> s[[ _pd ]] with
-    | (d, pd') => fun e =>
-      match e return
-        @sdenote (payload_desc' (S n')) (@SDenoted_payload_desc' (S n')) (d, pd')
-      with
-      | (v, e') =>
-        (eval_base_expr d v, eval_payload_expr' n' pd' e')
-      end
-    end e
-  end pd e.
-
-Definition eval_payload_expr (pd : payload_desc) (e : payload_expr pd) : s[[ pd ]] :=
-  eval_payload_expr' (projT1 pd) (projT2 pd) e.
-
-Inductive expr_desc : Set :=
+Inductive expr_desc :=
 | base_expr_d : desc -> expr_desc
 | msg_expr_d : expr_desc
 .
@@ -545,101 +687,264 @@ Instance SDenoted_expr_t : SDenoted expr_desc :=
 }.
 
 Inductive expr : expr_desc -> Type :=
-| Base :
-  forall d : desc,
-  base_expr d ->
-  expr (base_expr_d d)
-| MsgExpr :
-  forall tag,
-  payload_expr (lkup_tag tag) ->
-  expr msg_expr_d
+(* an expression evaluating to one constant *)
+| MEbase : forall d, base_expr d -> expr (base_expr_d d)
+(* an expression evaluating to a vector of constants *)
+| MEmsg : forall tag, payload_expr (lkup_tag tag) -> expr msg_expr_d
 .
 
+(* Within a handler, an expression may also refer to handler-specific things *)
+Inductive hdlr_expr : expr_desc -> Type :=
+| HEexpr : forall d, expr d -> hdlr_expr d
+| HEchan : hdlr_expr (base_expr_d fd_d)
+| HEparam : forall (i : fin (projT1 CPAY)),
+  hdlr_expr (base_expr_d (svec_ith (projT2 CPAY) i))
+(* Here should be HEkst or something to access a kstate variable *)
+.
+
+Section WITH_ENV.
+
+Variable ENV : s[[ ENVD ]].
+
+Fixpoint eval_base_expr (d : desc) (e : base_expr d) : s[[ d ]] :=
+  match e in base_expr _d return sdenote_desc _d with
+  | NLit n => n
+  | SLit s => s
+  | Var i => payload_ith ENVD ENV i
+  | UnOp t1 t2 op e =>
+    let v := eval_base_expr t1 e in
+    eval_unop op v
+  | BinOp t1 t2 t3 op e1 e2 =>
+    let v1 := eval_base_expr t1 e1 in
+    let v2 := eval_base_expr t2 e2 in
+    eval_binop op v1 v2
+  end.
+
+Fixpoint eval_payload_expr' (n : nat) :
+  forall (pd : vdesc' n), payload_expr' n pd -> s[[ pd ]] :=
+  let res n pd := payload_expr' n pd -> s[[ pd ]] in
+  match n as _n return
+    forall (pd : vdesc' _n), res _n pd
+  with
+  | O => fun _ _ => tt
+  | S n' => fun pd =>
+    let (d, pd') as _pd return res (S n') _pd := pd in
+    fun e =>
+      let (v, e') := e in
+      (eval_base_expr d v, eval_payload_expr' n' pd' e')
+  end.
+
+Definition eval_payload_expr (pd : vdesc) (e : payload_expr pd) : s[[ pd ]] :=
+  eval_payload_expr' (projT1 pd) (projT2 pd) e.
+
 Definition eval_expr (d : expr_desc) (e : expr d) : s[[ d ]] :=
-  match e in expr _d return s[[ _d ]] with
-  | Base t e => eval_base_expr t e
-  | MsgExpr t pe =>
-    let p := eval_payload_expr (lkup_tag t) pe in
+  match e with
+  | MEbase d' e' => eval_base_expr d' e'
+  | MEmsg t pl =>
+    let p := eval_payload_expr (lkup_tag t) pl in
     {| tag := t; pay := p |}
   end.
 
-Inductive cmd : Type :=
-| Send : base_expr fd_d -> expr msg_expr_d -> cmd
+Definition eval_hdlr_expr (d : expr_desc) (e : hdlr_expr d) : s[[ d ]] :=
+  match e with
+  | HEexpr d' e' => eval_expr d' e'
+  | HEchan => CFD
+  | HEparam i => msg_param_i i
+  end.
+
+Inductive cmd (e : expr_desc -> Type) : Type :=
+| Send : e (base_expr_d fd_d) -> expr msg_expr_d -> cmd e
 .
 
-Definition kstate_run_cmd (s : kstate) (c : cmd) : kstate :=
-  match c with
-  | Send fe me =>
-    let f := eval_base_expr _ fe in
-    let m := eval_expr _ me in
-    let tr := ktr s in
-    {| components := components s
-     ; ktr := tr ~~~ KSend f m :: tr
-     |}
-  end.
+Definition init_cmd := cmd expr.
 
-Definition prog : Type :=
-  list cmd.
+Definition init_prog := list init_cmd.
 
-Fixpoint kstate_run_prog (s : kstate) (p : prog) : kstate :=
-  match p with
-  | c :: cs => kstate_run_prog (kstate_run_cmd s c) cs
-  | nil => s
-  end.
+Definition hdlr_cmd := cmd hdlr_expr.
+
+Definition hdlr_prog := list hdlr_cmd.
 
 End WITH_ENV.
 
-Definition handler : Type :=
-  forall m : msg, prog m.
+Record init_state :=
+{ init_comps : list fd
+; init_ktr   : [KTrace]%type
+; init_env   : s[[ ENVD ]]
+; init_kst   : s[[ KST_DESC_ ]]
+}.
+
+Definition init_state_run_cmd (s : init_state) : init_cmd -> init_state :=
+  let (cs, tr, e, st) := s in
+  fun c =>
+    match c with
+    | Send fe me =>
+      let f := eval_expr e _ fe in
+      let m := eval_expr e _ me in
+      {| init_comps := cs
+       ; init_ktr   := tr ~~~ KSend f m :: tr
+       ; init_env   := e
+       ; init_kst   := st
+      |}
+    end.
+
+Fixpoint init_state_run_prog (s : init_state) (p : init_prog) : init_state :=
+  match p with
+  | c :: cs => init_state_run_prog (init_state_run_cmd s c) cs
+  | nil => s
+  end.
+
+Record hdlr_state :=
+{ hdlr_kst : kstate
+; hdlr_env : s[[ ENVD ]]
+}.
+
+(* This should probably move out once the environment can change *)
+Definition hdlr_state_run_cmd (s : hdlr_state) : hdlr_cmd -> hdlr_state :=
+  let (s', env) := s in
+  let (cs, tr, st, fd) := s' in
+  fun c =>
+    match c with
+    | Send fe me =>
+      let f := eval_hdlr_expr env _ fe in
+      let m := eval_expr env _ me in
+      {| hdlr_kst :=
+           {| kcs := cs
+            ; ktr := tr ~~~ KSend f m :: tr
+            ; kst := st
+            ; kfd := fd
+            |}
+       ; hdlr_env := env
+      |}
+    end.
+
+Fixpoint hdlr_state_run_prog (s : hdlr_state) (p : hdlr_prog) : hdlr_state :=
+  match p with
+  | nil => s
+  | c::cs => hdlr_state_run_prog (hdlr_state_run_cmd s c) cs
+  end.
+
+Axiom devnull : fd.
+
+Axiom devnull_open : emp ==> open devnull.
+
+Fixpoint default_payload' (n : nat) :
+  forall (v : vdesc' n), sdenote_vdesc' n v :=
+  match n with
+  | O    => fun _ => tt
+  | S n' => fun v =>
+    match v with
+    | (d, v') =>
+      ( match d as _d return sdenote_desc _d with
+        | num_d => FALSE
+        | str_d => nil
+        | fd_f  => devnull
+        end
+      , default_payload' n' v')
+    end
+  end.
+
+Definition default_payload (v : vdesc) : s[[ v ]] :=
+  default_payload' (projT1 v) (projT2 v).
+
+Fixpoint kstate_run_prog (s : kstate) (p : hdlr_prog) : kstate :=
+  let hs :=
+    {| hdlr_kst := s
+     ; hdlr_env := default_payload ENVD
+     |} in
+  hdlr_kst (hdlr_state_run_prog hs p).
+
+End WITH_ENVD.
+End WITHIN_HANDLER.
+
+Variable INIT_ENVD : vdesc.
+Variable INIT_PROG : init_prog INIT_ENVD.
+
+Definition initial_init_state :=
+  {| init_comps := nil
+   ; init_ktr   := [nil]%inhabited
+   ; init_env   := default_payload INIT_ENVD
+   ; init_kst   := default_payload KST_DESC_
+   |}.
 
 Section WITH_HANDLER.
 
-Variable HANDLER : handler.
+Definition handlers := forall (m : msg), sigT (fun (vd : vdesc) => hdlr_prog m vd).
 
-Definition init_str := str_of_string "test/echo-00/test.py".
+Variable HANDLERS : handlers.
+
+Fixpoint payload_fds' (n : nat) :
+  forall (v : vdesc' n), sdenote_vdesc' n v -> list fd :=
+  match n with
+  | 0 => fun _ _ => nil
+  | S n' => fun v =>
+    let (d, v') as _v return (sdenote_vdesc' (S n') _v -> list fd) := v in
+    match d with
+    | fd_d => fun vv =>
+      let (vd, vv') := vv in
+      vd :: payload_fds' n' v' vv'
+    | _ => fun vv =>
+      let (_, vv') := vv in
+      payload_fds' n' v' vv'
+    end
+  end.
+
+Definition payload_fds (v : vdesc) : s[[ v ]] -> list fd :=
+  payload_fds' (projT1 v) (projT2 v).
 
 Inductive Reach : kstate -> Prop :=
 | Reach_init :
-  forall f,
-  Reach
-    {| components := f :: nil
-     ; ktr := [KExec init_str nil f :: nil]
-     |}
+  forall s,
+  s = init_state_run_prog INIT_ENVD initial_init_state INIT_PROG ->
+  Reach {| kcs := init_comps _ s
+         ; ktr := init_ktr _ s
+         ; kst := init_kst _ s
+         ; kfd := payload_fds _ (init_env _ s)
+         |}
 | Reach_valid :
-  forall s f m tr s',
+  forall s f m tr s' s'',
   msg_fds_ok s m ->
-  let cs := components s in
+  let cs := kcs s in
   ktr s = [tr]%inhabited ->
   Reach s ->
-  s' = {| components := cs
+  s' = {| kcs := cs
         ; ktr := [KRecv f m :: KSelect cs f :: tr]
+        ; kst := kst s
+        ; kfd := kfd s
         |} ->
-  Reach (kstate_run_prog f m s' (HANDLER m))
+  s'' = kstate_run_prog f m (projT1 (HANDLERS m)) s' (projT2 (HANDLERS m)) ->
+  Reach {| kcs := kcs s''
+         ; ktr := ktr s''
+         ; kst := kst s''
+         ; kfd := kfd s'' ++ payload_fds _ (pay m)
+         |}
 | Reach_bad_fds :
   forall s f m tr,
-  let cs := components s in
+  let cs := kcs s in
   ~ msg_fds_ok s m ->
   ktr s = [tr]%inhabited ->
   Reach s ->
-  Reach {| components := cs
-        ; ktr := [KRecv f m :: KSelect cs f :: tr]
-        |}
+  Reach {| kcs := cs
+         ; ktr := [KRecv f m :: KSelect cs f :: tr]
+         ; kst := kst s
+         ; kfd := kfd s ++ payload_fds _ (pay m)
+         |}
 | Reach_bogus :
   forall s f bmsg tr,
-  let cs := components s in
+  let cs := kcs s in
   ktr s = [tr]%inhabited ->
   Reach s ->
   Reach
-    {| components := cs
+    {| kcs := cs
      ; ktr := [KBogus f bmsg :: KSelect cs f :: tr]
+     ; kst := kst s
+     ; kfd := kfd s
      |}
 .
 
 Definition kstate_inv s : hprop :=
   tr :~~ ktr s in emp
-  * traced (expand_ktrace tr)
-  * [Reach s]
-  * all_bound (components s)
+  * traced (expand_ktrace tr) * [Reach s]
+  * all_open (kcs s) * all_open (kfd s)
   .
 
 Ltac isolate t :=
@@ -649,25 +954,46 @@ Ltac isolate t :=
     apply himp_split
   end.
 
-Ltac bounds_packing :=
+Ltac opens_packing :=
   match goal with
   | [ |- ?lhs ==> ?rhs ] =>
-    match lhs with context [ all_bound_drop ?cs ?c ] =>
-      isolate (bound c * all_bound_drop cs c ==> all_bound cs);
-      [ apply repack_all_bound | ]
+    match lhs with context [ all_open_drop ?cs ?c ] =>
+      isolate (open c * all_open_drop cs c ==> all_open cs);
+      [ apply repack_all_open | ]
     end
 
   | [ |- ?lhs ==> ?rhs ] =>
-    match rhs with context [ all_bound_drop ?cs ?c ] =>
-      isolate (all_bound cs ==> bound c * all_bound_drop cs c);
-      [ apply unpack_all_bound | ]
+    match rhs with context [ all_open_drop ?cs ?c ] =>
+      isolate (all_open cs ==> open c * all_open_drop cs c);
+      [ apply unpack_all_open | ]
     end
 
   | [ |- ?lhs ==> ?rhs ] =>
-    match lhs with context [ all_bound_drop ?cs ?c ] =>
-    match rhs with context [ all_bound_drop ?cs ?d ] =>
-      isolate (bound c * all_bound_drop cs c ==> bound d * all_bound_drop cs d);
-      [ eapply himp_trans; [ apply repack_all_bound | apply unpack_all_bound ] | ]
+    match lhs with context [ all_open_drop ?cs ?c ] =>
+    match rhs with context [ all_open_drop ?cs ?d ] =>
+      isolate (open c * all_open_drop cs c ==> open d * all_open_drop cs d);
+      [ eapply himp_trans; [ apply repack_all_open | apply unpack_all_open ] | ]
+    end
+    end
+
+  | [ |- ?lhs ==> ?rhs ] =>
+    match lhs with context [ all_open_payload_drop ?f ?p ] =>
+      isolate (open f * all_open_payload_drop f p ==> all_open_payload p);
+      [ apply repack_all_open_payload | ]
+    end
+
+  | [ |- ?lhs ==> ?rhs ] =>
+    match rhs with context [ all_open_payload_drop ?f ?p ] =>
+      isolate (all_open_payload p ==> open f * all_open_payload_drop f p);
+      [ apply unpack_all_open_payload | ]
+    end
+
+  | [ |- ?lhs ==> ?rhs ] =>
+    match lhs with context [ all_open_payload_drop ?f ?p ] =>
+    match rhs with context [ all_open_payload_drop ?g ?p ] =>
+      isolate (open f * all_open_payload_drop f p ==> open g * all_open_drop g p);
+      [ eapply himp_trans;
+        [ apply repack_all_open_payload | apply unpack_all_open_payload ] | ]
     end
     end
 end.
@@ -689,8 +1015,7 @@ Ltac uninhabit :=
 
 Ltac misc :=
   match goal with
-  | [ |- Reach _ ] =>
-      econstructor; eauto
+  | [ |- Reach _ ] => econstructor; eauto
   end.
 
 Ltac unfoldr :=
@@ -699,11 +1024,183 @@ Ltac unfoldr :=
 Ltac simplr :=
   sep';
   try uninhabit;
-  try bounds_packing;
+  try opens_packing;
   try misc.
 
 Ltac sep'' :=
   sep unfoldr simplr.
+
+Lemma eval_base_expr_fd :
+  forall l d envd e v env,
+  env_fds_in l envd env ->
+  eval_base_expr envd env d e = v ->
+  match d as _d return (s[[ _d ]] -> Prop) with
+  | fd_d => fun f => In f l
+  | _ => fun _ => True
+  end v.
+Proof.
+  induction e; try tauto; intros vd env OK E; simpl in *.
+  subst. exact (OK i).
+  now destruct u.
+  now destruct b.
+Qed.
+
+Lemma eval_expr_fd :
+  forall l d envd e v env,
+  env_fds_in l envd env ->
+  eval_expr envd env d e = v ->
+  match d as _d return (sdenote_expr_desc _d -> Prop) with
+  | base_expr_d fd_d => fun f => In f l
+  | _ => fun _ => True
+  end v.
+Proof.
+  intros l d envd. induction e; intros vd env OK E; simpl in *.
+  destruct b; try tauto; simpl in *.
+  subst. exact (OK i).
+  now destruct u.
+  now destruct b1.
+  exact I.
+Qed.
+
+Theorem eval_expr_fd_in_payload : forall envd d fe v s,
+  eval_expr envd (init_env envd s) d fe = v ->
+  match d as _d return sdenote_expr_desc _d -> Prop with
+  | base_expr_d fd_d => fun f => fd_in_payload f envd (init_env envd s)
+  | _ => fun _ => True
+  end v.
+Proof.
+  intros envd d.
+  destruct fe; intros v s E; intuition simpl in *.
+  destruct b as []_eqn; intuition simpl in *. subst.
+  pose proof (
+    shvec_ith_in sdenote_desc desc_eqdec UIP_refl_desc (projT2 envd)
+    (init_env envd s) i
+  ).
+  destruct envd as [n envd]. simpl in *.
+  unfold payload_ith.
+  generalize dependent (
+    shvec_ith sdenote_desc envd
+      (init_env (existT (fun n0 : nat => vdesc' n0) n envd) s) i
+  ).
+  intros.
+  destruct (svec_ith envd i); tauto.
+  now destruct u.
+  now destruct b0.
+Qed.
+
+Definition init_invariant {envd} (s : init_state envd) :=
+  all_open (init_comps _ s)
+  * all_open_payload (init_env _ s).
+
+Definition run_init_cmd :
+  forall (envd : vdesc) (s : init_state envd) (c : init_cmd envd),
+  STsep (tr :~~ init_ktr envd s in
+          init_invariant s * traced (expand_ktrace tr))
+        (fun s' : init_state envd => tr :~~ init_ktr envd s' in
+          init_invariant s' * traced (expand_ktrace tr) * [s' = init_state_run_cmd envd s c]).
+Proof.
+  intros; refine (
+    let cs := init_comps _ s in
+    let tr := init_ktr _ s in
+    let e  := init_env _ s in
+    let st := init_kst _ s in
+    match c with
+    | Send fe me =>
+      (* /!\ We lose track of the let-open equalities if existentials remain,
+         make sure that Coq can infer _all_ the underscores. *)
+      let f := eval_expr _ e _ fe in
+      let m := eval_expr _ e _ me in
+      send_msg f m (tr ~~~ expand_ktrace tr)
+      <@> all_open cs * all_open_payload_drop f e;;
+
+      let tr := tr ~~~ KSend f m :: tr in
+      {{ Return {| init_comps := cs
+                 ; init_ktr   := tr
+                 ; init_env   := e
+                 ; init_kst   := st
+                 |} }}
+    end
+  ); unfold init_invariant, cs, e; sep''.
+  pose proof eval_expr_fd_in_payload as E.
+  specialize (E _ _ fe f s (Logic.eq_refl f)). now simpl in E.
+  pose proof eval_expr_fd_in_payload as E.
+  specialize (E _ _ fe f s (Logic.eq_refl f)). now simpl in E.
+  apply himp_pure'.
+  unfold init_state_run_cmd. destruct s. simpl.
+  sep''. unfold f, m, e. simpl in *. sep''.
+  (* dirty proof, could be made nicer... *)
+Qed.
+
+(* that seems wrong and unneeded
+Fixpoint init_env_fds_ok' (n : nat) : forall (v : vdesc' n), sdenote_vdesc' n v -> hprop.
+Proof.
+  destruct n as [|n']. exact (fun _ _ => emp).
+  intros v. destruct v as [d v']. destruct d.
+  intros vv. destruct vv as (vd, vv'). exact (init_env_fds_ok' n' v' vv').
+  intros vv. destruct vv as (vd, vv'). exact (init_env_fds_ok' n' v' vv').
+  intros vv. destruct vv as (vd, vv'). exact (open vd * init_env_fds_ok' n' v' vv').
+Qed.
+
+(* is this needed? *)
+Fixpoint init_env_fds_ok'' (n : nat) :
+  forall (v : vdesc' n), sdenote_vdesc' n v -> hprop :=
+  match n with
+  | 0 => fun _ _ => emp
+  | S n0 =>
+    fun v =>
+    let (d, v') as p return (sdenote_vdesc' (S n0) p -> hprop) := v in
+    fun vv =>
+    let (vd, _) := vv in
+    match d as d0 return (s[[d0]] -> hprop) with
+    | fd_d => fun vd => open vd
+    | _ => fun _ => emp
+    end vd
+  end
+.
+*)
+
+Definition run_init_prog :
+  forall (envd : vdesc) (s : init_state envd) (p : init_prog envd),
+  STsep (tr :~~ init_ktr envd s in
+          init_invariant s * traced (expand_ktrace tr))
+        (fun s' : init_state envd => tr :~~ init_ktr envd s' in
+          init_invariant s' * traced (expand_ktrace tr) * [s' = init_state_run_prog envd s p]).
+Proof.
+  intros; refine (
+    Fix2
+      (fun p s => tr :~~ init_ktr envd s in
+        init_invariant s * traced (expand_ktrace tr))
+      (fun p s (s' : init_state envd) => tr :~~ init_ktr envd s' in
+        init_invariant s' * traced (expand_ktrace tr) * [s' = init_state_run_prog envd s p])
+      (fun self p s =>
+        match p with
+        | nil => {{ Return s }}
+        | c::cs =>
+          s' <- run_init_cmd envd s c;
+          s'' <- self cs s' <@> [s' = init_state_run_cmd envd s c];
+          {{ Return s'' }}
+        end
+      )
+    p s
+  ); sep''.
+Qed.
+
+Theorem all_open_default_payload : forall henv,
+  emp ==> all_open_payload (default_payload henv).
+Proof.
+  intros [n envd]. induction n.
+  unfold all_open_payload, all_open_payload'. now simpl.
+  destruct envd as [d envd']. unfold default_payload. simpl.
+  destruct d.
+  exact (IHn envd').
+  exact (IHn envd').
+  unfold all_open_payload, all_open_payload'. simpl.
+  isolate (emp ==> open devnull). exact devnull_open.
+  exact (IHn envd').
+Qed.
+
+Axiom all_open_payload_to_all_open : forall v p,
+  all_open_payload p ==> all_open (payload_fds v p).
 
 Definition kinit :
   forall (_ : unit),
@@ -711,69 +1208,129 @@ Definition kinit :
         (fun s => kstate_inv s).
 Proof.
   intros; refine (
-    let tr := [nil]%inhabited in
-    c <- exec init_str nil tr;
-    let tr := tr ~~~ KExec init_str nil c :: nil in
-    {{Return {|components := c :: nil; ktr := tr|}}}
-  );
-  sep''.
+    let s := initial_init_state in
+    s' <- run_init_prog _ s INIT_PROG;
+    {{ Return {| kcs := init_comps _ s'
+               ; ktr := init_ktr _ s'
+               ; kst := init_kst _ s'
+               ; kfd := nil ++ payload_fds _ (init_env _ s')
+               |}
+     }}
+  ); unfold init_invariant; sep''.
+  apply all_open_default_payload.
+  apply all_open_payload_to_all_open.
 Qed.
 
-Definition run_cmd :
-  forall (cfd : fd) (cm : msg) (s : kstate) (c : cmd cm),
-  STsep (tr :~~ ktr s in
-          traced (expand_ktrace tr) * all_bound (components s) *
-          [In cfd (components s)] * [msg_fds_ok s cm])
-        (fun s' : kstate => tr :~~ ktr s' in
-          traced (expand_ktrace tr) * all_bound (components s') *
-          [In cfd (components s')] * [msg_fds_ok s' cm] * [kstate_run_cmd cfd cm s c = s']).
+(*
+Definition run_init_cmd :
+  forall (envd : vdesc) (s : init_state envd) (c : init_cmd envd),
+  STsep (tr :~~ init_ktr envd s in
+          init_invariant s * traced (expand_ktrace tr))
+        (fun s' : init_state envd => tr :~~ init_ktr envd s' in
+          init_invariant s' * traced (expand_ktrace tr) * [s' = init_state_run_cmd envd s c]).
+*)
+
+Definition env_fds_ok envd (hs : hdlr_state envd) :=
+  env_fds_in (kfd (hdlr_kst envd hs)) envd (hdlr_env envd hs).
+
+Theorem eval_hdlr_expr_fd_in : forall cfd cm envd d fe v (s : hdlr_state envd),
+  let (kst, env) := s in
+  env_fds_ok envd s ->
+  msg_fds_ok kst cm ->
+  In cfd (kcs kst) ->
+  eval_hdlr_expr cfd cm envd env d fe = v ->
+  match d as _d return sdenote_expr_desc _d -> Prop with
+  | base_expr_d fd_d => fun f => In f (kcs kst) \/ In f (kfd kst)
+  | _ => fun _ => True
+  end v.
+Proof.
+  intros until s. destruct s as [kst env]. simpl. intros F M I E. subst.
+  destruct fe; simpl in *; try tauto.
+  destruct e; simpl in *; try tauto.
+  destruct b; simpl in *; try tauto.
+  specialize (F i). simpl in F.
+  generalize dependent (payload_ith envd env i).
+  destruct (svec_ith (projT2 envd) i); tauto.
+  now destruct u.
+  now destruct b1.
+  specialize (M i). simpl in *.
+  generalize dependent (msg_param_i cm i).
+  destruct (svec_ith (projT2 (lkup_tag (tag cm))) i); tauto.
+Qed.
+
+Definition hdlr_invariant {envd} (cfd : fd) (cm : msg) (s : hdlr_state envd) :=
+  let (kst, env) := s in
+  all_open (kcs kst ++ kfd kst)
+  * all_open_payload (pay cm) (* this might become problematic *)
+  * [In cfd (kcs kst)] * [msg_fds_ok kst cm] * [env_fds_ok envd s]
+.
+
+Definition run_hdlr_cmd :
+  forall (cfd : fd) (cm : msg) (envd : vdesc) (s : hdlr_state envd) (c : hdlr_cmd cm envd),
+  STsep (tr :~~ ktr (hdlr_kst _ s) in
+          hdlr_invariant cfd cm s * traced (expand_ktrace tr))
+        (fun s' : hdlr_state envd => tr :~~ ktr (hdlr_kst _ s') in
+          hdlr_invariant cfd cm s' * traced (expand_ktrace tr)
+          * [s' = hdlr_state_run_cmd cfd cm envd s c]).
 Proof.
   intros; refine (
-    let comps := components s in
-    let tr := ktr s in
+    (* you lose the equations if you try to let (st, env, fds) := s *)
+    let st := hdlr_kst _ s in
+    let env := hdlr_env _ s in
+    let comps := kcs st in
+    let tr := ktr st in
+    let fds := kfd st in
     match c with
     | Send fe me =>
-      let f := eval_base_expr cfd cm _ fe in
-      let m := eval_expr cfd cm _ me in
-      send_msg f ExecPerms m
+      let f := eval_hdlr_expr cfd cm _ env _ fe in
+      let m := eval_expr envd env _ me in
+      send_msg f m
       (tr ~~~ expand_ktrace tr)
-      <@> all_bound_drop comps f * [In cfd comps] * [msg_fds_ok s cm];;
+      <@> all_open_drop (comps ++ fds) f * all_open_payload (pay cm)
+      * [In cfd comps] * [msg_fds_ok st cm] * [env_fds_ok envd s];;
 
       let tr := tr ~~~ KSend f m :: tr in
-      {{Return {|components := comps; ktr := tr|}}}
+      {{Return {| hdlr_kst := {| kcs := comps ; ktr := tr ; kst := kst st ; kfd := fds |}
+                ; hdlr_env := env
+                |}
+      }}
     end
-  );
+  ); unfold env, fds, hdlr_invariant in *; clear env fds; sep fail idtac;
+  pose proof (eval_hdlr_expr_fd_in cfd cm _ _ fe f s) as E;
+  destruct s as (kst, env).
   sep''.
-  eapply (base_expr_fd_in s cfd cm fd_d); eauto.
-  eapply (base_expr_fd_in s cfd cm fd_d); eauto.
+  sep''.
+  apply himp_pure'. destruct kst as (kcs, ktr, kst, kfd). simpl in *.
+  unfold comps in *. clear comps. sep''.
+  apply himp_pure'. destruct kst as (cs, ktr, kst, kfd). simpl in *.
+  unfold comps in *. clear comps. sep''.
+  (* so ugly... *)
 Qed.
 
-Definition run_prog :
-  forall (cfd : fd) (cm : msg) (s : kstate) (p : prog cm),
-  STsep (tr :~~ ktr s in
-          traced (expand_ktrace tr) * all_bound (components s) *
-          [In cfd (components s)] * [msg_fds_ok s cm])
-        (fun s' : kstate => tr :~~ ktr s' in
-          traced (expand_ktrace tr) * all_bound (components s') *
-          [In cfd (components s')] * [msg_fds_ok s' cm] * [kstate_run_prog cfd cm s p = s']).
+Definition run_hdlr_prog :
+  forall (cfd : fd) (cm : msg) (envd : vdesc) (s : hdlr_state envd) (p : hdlr_prog cm envd),
+  STsep (tr :~~ ktr (hdlr_kst _ s) in
+          hdlr_invariant cfd cm s * traced (expand_ktrace tr))
+        (fun s' : hdlr_state envd => tr :~~ ktr (hdlr_kst _ s') in
+          hdlr_invariant cfd cm s' * traced (expand_ktrace tr)
+          * [s' = hdlr_state_run_prog cfd cm envd s p]).
 Proof.
   intros; refine (
     Fix2
-      (fun p s =>
-        tr :~~ ktr s in
-          traced (expand_ktrace tr) * all_bound (components s) *
-          [In cfd (components s)] * [msg_fds_ok s cm])
-      (fun p s (s' : kstate) =>
-        tr :~~ ktr s' in
-          traced (expand_ktrace tr) * all_bound (components s') *
-          [In cfd (components s')] * [msg_fds_ok s' cm] * [kstate_run_prog cfd cm s p = s'])
+      (fun p (s : hdlr_state envd) =>
+        tr :~~ ktr (hdlr_kst _ s) in
+          hdlr_invariant cfd cm s * traced (expand_ktrace tr))
+      (fun p s (s' : hdlr_state envd) =>
+        tr :~~ ktr (hdlr_kst _ s') in
+          hdlr_invariant cfd cm s' * traced (expand_ktrace tr)
+          * [s' = hdlr_state_run_prog cfd cm envd s p])
       (fun self p s =>
         match p with
         | nil =>
           {{ Return s }}
         | c::cs =>
-          s' <- run_cmd cfd cm s c;
-          s'' <- self cs s' <@> [kstate_run_cmd cfd cm s c = s'];
+          s' <- run_hdlr_cmd cfd cm envd s c;
+          s'' <- self cs s' <@> [hdlr_state_run_cmd cfd cm envd s c = s'];
           {{ Return s'' }}
         end)
     p s
@@ -781,47 +1338,120 @@ Proof.
   sep''.
 Qed.
 
+Theorem all_open_concat : forall a b,
+  all_open a * all_open b ==> all_open (a ++ b).
+Proof.
+  induction a.
+  simpl. sep'.
+  simpl. sep'.
+Qed.
+
+Theorem all_open_unconcat : forall a b,
+  all_open (a ++ b) ==> all_open a * all_open b.
+Proof.
+  induction a.
+  simpl. sep'.
+  simpl. sep'.
+Qed.
+
+Axiom in_devnull_default_payload: forall henv l,
+  env_fds_in (devnull :: l) henv (default_payload henv).
+
 Definition kbody:
   forall s,
   STsep (kstate_inv s)
         (fun s' => kstate_inv s').
 Proof.
-  intro kst.
-  remember (components kst) as comps.
+  intro s.
   refine (
-    let tr := ktr kst in
-    c <- select comps
+    let cs := kcs s in
+    let tr := ktr s in
+    let st := kst s in
+    let fd := kfd s in
+    c <- select cs
     (tr ~~~ expand_ktrace tr)
-    <@> (tr ~~ [Reach kst] * all_bound comps);
+    <@> (tr ~~ [Reach s] * all_open cs * all_open fd);
 
-    let tr := tr ~~~ KSelect comps c :: tr in
-    mm <- recv_msg c ExecPerms
+    let tr := tr ~~~ KSelect cs c :: tr in
+    mm <- recv_msg c
     (tr ~~~ expand_ktrace tr)
-    <@> (tr ~~ [In c comps] * [Reach kst] * all_bound_drop comps c);
+    <@> (tr ~~ [In c cs] * [Reach s] * all_open_drop cs c * all_open fd);
 
     match mm with
     | inl m =>
       let tr := tr ~~~ KRecv c m :: tr in
-      let ck := msg_fds_ck kst m in
+      let ck := msg_fds_ck s m in
       match ck as ck' return ck = ck' -> _ with
       | left _ => fun _ =>
-        let s' := {|components := comps; ktr := tr|} in
-        s'' <- run_prog c m s' (HANDLER m) <@> [Reach kst];
-        {{Return s''}}
+        let henv  := projT1 (HANDLERS m) in
+        let hprog := projT2 (HANDLERS m) in
+        let s' := {| hdlr_kst := {| kcs := cs
+                                  ; ktr := tr
+                                  ; kst := st
+                                  ; kfd := (*devnull ::*) fd |}
+                   ; hdlr_env := default_payload henv
+                   |}
+        in
+        s'' <- run_hdlr_prog c m henv s' hprog <@> [Reach s];
+        (* we need to add the payload open fds to kfd so as not to keep track of any
+           linear resource *)
+        let s''' := {| hdlr_kst := {| kcs := kcs (hdlr_kst _ s'')
+                                    ; ktr := ktr (hdlr_kst _ s'')
+                                    ; kst := kst (hdlr_kst _ s'')
+                                    ; kfd := kfd (hdlr_kst _ s'') ++ payload_fds _ (pay m) |}
+                     ; hdlr_env := hdlr_env _ s''
+                     |}
+        in
+        {{ Return (hdlr_kst _ s''') }}
       | right _ => fun _ =>
-        {{Return {|components := comps; ktr := tr|}}}
+        {{Return {|kcs := cs; ktr := tr; kfd := fd ++ payload_fds _ (pay m)|}}}
       end (refl_equal ck)
     | inr m =>
       let tr := tr ~~~ KBogus c m :: tr in
-      {{Return {|components := comps; ktr := tr|}}}
+      {{Return {|kcs := cs; ktr := tr; kfd := fd|}}}
     end
-  );
+  ); unfold hdlr_invariant in *; sep''.
+
+  isolate (
+    all_open_drop cs c * open c * all_open fd
+    ==> all_open (cs ++ (*devnull ::*) fd)
+  ).
+
+  apply himp_trans with (Q := all_open cs * all_open fd); sep''.
+  apply himp_trans with (Q := all_open cs * all_open ((*devnull ::*) fd)).
+  sep''. (*apply devnull_open.*) apply all_open_concat.
+  apply himp_pure'. unfold env_fds_ok. simpl. admit. (*apply in_devnull_default_payload.*)
+
+  destruct (hdlr_state_run_prog c m henv s' hprog) as [kst'' env'']_eqn.
+  simpl in *. sep''.
+  isolate (
+    all_open (kcs kst'' ++ kfd kst'') * all_open_payload (pay m)
+    ==> all_open (kcs kst'') * all_open (kfd kst'' ++ payload_fds _ (pay m))
+  ).
+  apply himp_trans with
+  (Q := all_open (kcs kst'') * all_open (kfd kst'') * all_open_payload (pay m)); sep''.
+  apply all_open_unconcat.
+  apply himp_trans with
+  (Q := all_open (kfd kst'') * all_open (payload_fds _ (pay m))); sep''.
+  apply all_open_payload_to_all_open.
+  apply all_open_concat.
+
+  sep''. constructor; auto.
+  eapply Reach_valid with (s := s) (s' := (hdlr_kst _ s')); eauto.
+  unfold s'. simpl. unfold cs, st, fd. sep''.
+
+  unfold kstate_run_prog. simpl.
+  unfold s' in Heqh.
+  unfold henv, hprog in Heqh. rewrite Heqh. now simpl.
+
+  isolate (
+    all_open_payload (pay m) * all_open fd ==>
+    all_open (fd ++ payload_fds (lkup_tag (tag m)) (pay m))
+  ).
+  eapply himp_trans; [ | apply all_open_concat ]. sep''.
+  apply all_open_payload_to_all_open.
+
   sep''.
-  subst v; sep''.
-  econstructor; eauto.
-  unfold s' in *; rewrite <- H6.
-  eapply (Reach_valid kst); eauto.
-  f_equal; auto. sep''.
 Qed.
 
 Definition kloop:
@@ -861,9 +1491,13 @@ End WITH_HANDLER.
 End WITH_PAYLOAD_DESC_VEC.
 
 Record spec :=
-{ NB_MSG   : nat
-; PAY_DESC : payload_desc_vec NB_MSG
-; HANDLERS : handler (PDV:=PAY_DESC)
+{ NB_MSG    : nat
+; PAY_DESC  : vvdesc NB_MSG
+; INIT_ENVD : vdesc
+; INIT      : @init_prog NB_MSG PAY_DESC INIT_ENVD
+; KST_DESC  : vdesc
+; HANDLERS  : handlers (VVD := PAY_DESC)
 }.
 
-Definition mk_main (s : spec) := main (HANDLERS s).
+Definition mk_main (s : spec) :=
+  @main _ (PAY_DESC s) _ (projT2 (KST_DESC s)) _ (INIT s) (HANDLERS s).
