compiler/dsl/coq/ReflexIO.v
@@ -26,26 +26,17 @@ Definition Trace : Set := list Action.
 
 Axiom traced : Trace -> hprop.
 
-Inductive Perm : Set :=
-  RecvP | SendP | RecvFDP | SendFDP.
-
-Definition ExecPerms : list Perm :=
-  RecvP :: SendP :: RecvFDP :: SendFDP :: nil.
-
-Definition CallPerms : list Perm :=
-  RecvP :: RecvFDP :: nil.
-
-Axiom open : fd -> list Perm -> hprop.
+Axiom open : fd -> hprop.
 
 Axiom exec :
   forall (prog : str) (args : list str) (tr : [Trace]),
     STsep (tr ~~ traced tr)
-          (fun f : fd => tr ~~ open f ExecPerms * traced (Exec prog args f :: tr)).
+          (fun f : fd => tr ~~ open f * traced (Exec prog args f :: tr)).
 
 Axiom call :
   forall (prog : str) (args : list str) (tr : [Trace]),
   STsep (tr ~~ traced tr)
-        (fun f : fd => tr ~~ open f CallPerms * traced (Call prog args f :: tr)).
+        (fun f : fd => tr ~~ open f * traced (Call prog args f :: tr)).
 
 (* TODO add non-empty precondition *)
 (* TODO add open w/ recv perms precondition *)
@@ -55,25 +46,25 @@ Axiom select :
         (fun f : fd => tr ~~ traced (Select fs f :: tr) * [In f fs]).
 
 Axiom recv :
-  forall (f : fd) (ps : list Perm) (n : num) (tr : [Trace]),
-  STsep (tr ~~ traced tr * open f ps * [In RecvP ps])
-        (fun s : str => tr ~~ traced (Recv f s :: tr) * open f ps *
+  forall (f : fd) (n : num) (tr : [Trace]),
+  STsep (tr ~~ traced tr * open f)
+        (fun s : str => tr ~~ traced (Recv f s :: tr) * open f *
           [nat_of_num n = List.length s]).
 
 Axiom send :
-  forall (f : fd) (ps : list Perm) (s : str) (tr : [Trace]),
-  STsep (tr ~~ traced tr * open f ps * [In SendP ps])
-        (fun _ : unit => tr ~~ traced (Send f s :: tr) * open f ps).
+  forall (f : fd) (s : str) (tr : [Trace]),
+  STsep (tr ~~ traced tr * open f)
+        (fun _ : unit => tr ~~ traced (Send f s :: tr) * open f).
 
 Axiom recv_fd :
-  forall (f : fd) (ps : list Perm) (tr : [Trace]),
-  STsep (tr ~~ traced tr * open f ps * [In RecvFDP ps])
-        (fun f' : fd => tr ~~ traced (RecvFD f f' :: tr) * open f ps).
+  forall (f : fd) (tr : [Trace]),
+  STsep (tr ~~ traced tr * open f)
+        (fun f' : fd => tr ~~ traced (RecvFD f f' :: tr) * open f * open f').
 
 Axiom send_fd :
-  forall (f : fd) (ps : list Perm) (f' : fd) (tr : [Trace]),
-  STsep (tr ~~ traced tr * open f ps * [In SendFDP ps])
-        (fun _ : unit => tr ~~ traced (SendFD f f' :: tr) * open f ps).
+  forall (f : fd) (f' : fd) (tr : [Trace]),
+  STsep (tr ~~ traced tr * open f)
+        (fun _ : unit => tr ~~ traced (SendFD f f' :: tr) * open f).
 
 (* we use big endian to follow network order *)
 Definition RecvNum (f : fd) (n : num) : Trace :=
@@ -93,12 +84,12 @@ Definition SendStr (f : fd) (s : str) : Trace :=
   Send f s :: SendNum f (num_of_nat (List.length s)).
 
 Definition recv_num:
-  forall (f : fd) (ps : list Perm) (tr : [Trace]),
-  STsep (tr ~~ traced tr * open f ps * [In RecvP ps])
-        (fun n : num => tr ~~ traced (RecvNum f n ++ tr) * open f ps).
+  forall (f : fd) (tr : [Trace]),
+  STsep (tr ~~ traced tr * open f)
+        (fun n : num => tr ~~ traced (RecvNum f n ++ tr) * open f).
 Proof.
   intros; refine (
-    s <- recv f ps (Num "002" "000") tr;
+    s <- recv f (Num "002" "000") tr;
     match s with
     | h :: l :: nil =>
       {{ Return (Num l h) }}
@@ -110,14 +101,14 @@ Proof.
 Qed.
 
 Definition send_num:
-  forall (f : fd) (ps : list Perm) (n : num) (tr : [Trace]),
-  STsep (tr ~~ traced tr * open f ps * [In SendP ps])
-        (fun _ : unit => tr ~~ traced (SendNum f n ++ tr) * open f ps).
+  forall (f : fd) (n : num) (tr : [Trace]),
+  STsep (tr ~~ traced tr * open f)
+        (fun _ : unit => tr ~~ traced (SendNum f n ++ tr) * open f).
 Proof.
   intros; refine (
     match n with
     | Num l h =>
-      send f ps (h :: l :: nil) tr;;
+      send f (h :: l :: nil) tr;;
       {{ Return tt }}
     end
   );
@@ -125,13 +116,13 @@ Proof.
 Qed.
 
 Definition recv_str:
-  forall (f : fd) (ps : list Perm) (tr : [Trace]),
-  STsep (tr ~~ traced tr * open f ps * [In RecvP ps])
-        (fun s : str => tr ~~ traced (RecvStr f s ++ tr) * open f ps).
+  forall (f : fd) (tr : [Trace]),
+  STsep (tr ~~ traced tr * open f)
+        (fun s : str => tr ~~ traced (RecvStr f s ++ tr) * open f).
 Proof.
   intros; refine (
-    n <- recv_num f ps tr <@> [In RecvP ps];
-    s <- recv f ps n (tr ~~~ RecvNum f n ++ tr);
+    n <- recv_num f tr;
+    s <- recv f n (tr ~~~ RecvNum f n ++ tr);
     {{ Return s }}
   );
   sep'.
@@ -141,14 +132,14 @@ Proof.
 Qed.
 
 Definition send_str:
-  forall (f : fd) (ps : list Perm) (s : str) (tr : [Trace]),
-  STsep (tr ~~ traced tr * open f ps * [In SendP ps])
-        (fun (_ : unit) => tr ~~ traced (SendStr f s ++ tr) * open f ps).
+  forall (f : fd) (s : str) (tr : [Trace]),
+  STsep (tr ~~ traced tr * open f)
+        (fun (_ : unit) => tr ~~ traced (SendStr f s ++ tr) * open f).
 Proof.
   intros; refine (
     let n := num_of_nat (List.length s) in
-    send_num f ps n tr <@> [In SendP ps];;
-    send f ps s (tr ~~~ SendNum f n ++ tr);;
+    send_num f n tr;;
+    send f s (tr ~~~ SendNum f n ++ tr);;
     {{ Return tt }}
   );
   sep'.
@@ -157,28 +148,25 @@ Qed.
 (* prevent sep tactic from unfolding *)
 Global Opaque RecvNum SendNum RecvStr SendStr.
 
-Definition bound (f : fd) : hprop :=
-  open f ExecPerms.
-
-Fixpoint all_bound (fds : list fd) : hprop :=
+Fixpoint all_open (fds : list fd) : hprop :=
   match fds with
   | nil => emp
-  | f :: fs => bound f * all_bound fs
+  | f :: fs => open f * all_open fs
   end.
 
-Fixpoint all_bound_drop (fds : list fd) (drop : fd) : hprop :=
+Fixpoint all_open_drop (fds : list fd) (drop : fd) : hprop :=
   match fds with
   | nil => emp
   | f :: fs =>
     if fd_eq f drop
-      then all_bound fs
-      else bound f * all_bound_drop fs drop
+      then all_open fs
+      else open f * all_open_drop fs drop
   end.
 
-Lemma unpack_all_bound :
+Lemma unpack_all_open :
   forall fs f,
   In f fs ->
-  all_bound fs ==> bound f * all_bound_drop fs f.
+  all_open fs ==> open f * all_open_drop fs f.
 Proof.
   induction fs; simpl; intros. contradiction.
   destruct H; subst. rewrite fd_eq_true. apply himp_refl.
@@ -188,10 +176,10 @@ Proof.
   apply himp_comm_conc; auto.
 Qed.
 
-Lemma repack_all_bound :
+Lemma repack_all_open :
   forall fs f,
   In f fs ->
-  bound f * all_bound_drop fs f ==> all_bound fs.
+  open f * all_open_drop fs f ==> all_open fs.
 Proof.
   induction fs; simpl; intros. contradiction.
   destruct H; subst. rewrite fd_eq_true. apply himp_refl.
